Radical changes to FFI and correctness (broken)

projection/proofs/comms_ffiScript.sml
@@ -1,53 +1,132 @@
 open    HolKernel
         Parse
         bossLib
+        relationTheory
+        quotientTheory
         astBakeryTheory
+        payloadSemanticsTheory
         ffiTheory;
 
 val _ = new_theory "comms_ffi";
 
-val _ = type_abbrev("message" , “: proc # datum”);
+val _ = type_abbrev("message", “: proc # datum”);
+val _ = type_abbrev("queue" , “: message list”);
+val _ = type_abbrev("total_state" , “: proc # queue # network”);
 
-val _ = Datatype‘
-  comms_state = <| sent_messages    : message list ;
-                   receive_messages : message llist
-                 |>
+val _ = Datatype ‘
+ action = ASend proc datum
+          | ARecv proc datum
 ’;
+
+val (strans_rules,strans_ind,strans_cases) = Hol_reln
+‘
+  (* ARecv *)
+  (∀conf c q q1 ms mc q2 N.
+    (q = q1 ++ [(ms,mc)] ++ q2) ∧
+    EVERY (λ(p,_). p ≠ ms) q1 
+    ⇒ strans conf (c,q,N) (ARecv ms mc) (c, q1 ++ q2, N))
+
+  (* LTauL *)
+∧ (∀conf c q q' N N' N'' α.
+     trans conf N LTau N' ∧
+     strans conf (c,q,N') α (c,q',N'')
+     ⇒  strans conf (c,q,N) α (c,q',N''))
+
+  (* LTauR *)
+∧ (∀conf c q q' N N' N'' α.
+     strans conf (c,q,N) α (c,q',N') ∧
+     trans conf N' LTau N''
+     ⇒  strans conf (c,q,N) α (c,q',N''))
+
+  (* LSend *)
+∧ (∀conf c q q' N N' N'' sp d α.
+     trans conf N (LSend sp d c) N' ∧
+     strans conf (c,q++[(sp,d)],N') α (c,q',N'')
+     ⇒  strans conf (c,q,N) α (c,q',N''))
+
+  (* ASend *)
+∧ (∀conf c q N N' rp d.
+     trans conf N (LReceive c d rp) N'
+     ⇒  strans conf (c,q,N) (ASend rp d) (c,q,N'))
+’;
+
+val bisim_def =
+Define
+‘
+  bisim ts R = ∀p q α.
+                R p q ⇒
+                (∀p'. ts p α p' ⇒ (∃q'. ts q α q' ∧ R p' q')) ∧
+                (∀q'. ts q α q' ⇒ (∃p'. ts p α p' ∧ R p' q'))
+’;
+
+val bisimRel_def =
+Define
+‘
+  bisimRel ts p q = ∃R. bisim ts R ∧ R p q
+’;
+
+
+Theorem bisimRel_equivRel:
+  ∀ts. equivalence (bisimRel ts)
+Proof
+  rw[equivalence_def] >> cheat
+QED
+
+val ffi_eq_def =
+Define
+‘
+  ffi_eq conf = bisimRel (strans conf)
+’;
+
+Theorem ffi_eq_equivRel:
+  ∀conf. equivalence (ffi_eq conf)
+Proof
+  rw [ffi_eq_def,bisimRel_equivRel]
+  >- (rw[reflexive_def, bisimRel_def] >>
+      qexists_tac ‘$=’ >>
+      rw[bisim_def])
+  >- (rw[symmetric_def, bisimRel_def] >>
+      rw[EQ_IMP_THM] >>
+      qexists_tac ‘SC R’ >>
+      fs[bisim_def,SC_DEF] >>
+      metis_tac[])
+  >- (rw[transitive_def,bisimRel_def] >>
+      qexists_tac ‘λa c. ∃b. R a b ∧ R' b c’ >>
+      fs[bisim_def] >>
+      metis_tac[])
+QED
 
 val ffi_send_def =
     Define
     ‘
-        ffi_send net_state dest data =
-            Oracle_return (net_state with sent_messages updated_by (CONS (dest,data))) data
-    ’;
-
-val find_first_def =
-    Define
-    ‘
-    find_first P ll =
-        case $OLEAST (λn. ∃x. (LNTH n ll = SOME x) ∧ P x) of
-                SOME n => SOME (THE (LTAKE n ll), THE (LNTH n ll), THE (LDROP (SUC n) ll))
-            |   NONE   => NONE
+        ffi_send conf os dest data =
+          if (∃ns. strans conf os (ASend dest data) ns) then
+            Oracle_return (@ns. strans conf os (ASend dest data) ns) data
+          else
+            Oracle_final FFI_diverged
     ’;
 
 val ffi_receive_def =
     Define
     ‘
-        ffi_receive net_state src _ =
-            case find_first (λ(p,_). p = src) net_state.receive_messages of
-                    SOME (q1,(p,d),q2)  => Oracle_return (net_state with receive_messages := LAPPEND (fromList q1) q2) d
-                |   NONE                => Oracle_final FFI_diverged
+        ffi_receive conf os src _ =
+          if (∃p. strans conf os (ARecv src (FST p)) (SND p)) then
+            let (m,ns) = (@p. strans conf os (ARecv src (FST p)) (SND p)) in
+              Oracle_return ns m
+          else
+            Oracle_final FFI_diverged
     ’;
 
 val comms_ffi_oracle_def = Define
 ‘
-  comms_ffi_oracle name =
+  comms_ffi_oracle conf name =
     if name = "send" then
-        ffi_send
+        ffi_send conf
     else if name = "receive" then
-        ffi_receive
+        ffi_receive conf
     else
         (λ _ _ _. Oracle_final FFI_failed)
 ’;
+
 
 val _ = export_theory ();
